Veritas.Verifier.fst
@@ -18,16 +18,148 @@ open Veritas.Verifier.Defs
  *)
 
 (* Each entry of the verifier log *)
-type verifier_log_entry =
-  | MemoryOp: o:memory_op -> verifier_log_entry
-  | AddM: a:merkle_addr -> v:merkle_payload -> a':merkle_addr -> verifier_log_entry
-  | EvictM: a:merkle_addr -> a':merkle_addr -> verifier_log_entry
+type vlog_entry_thread =
+  | MemoryOp: o:memory_op -> vlog_entry_thread
+  | AddM: a:merkle_addr -> v:merkle_payload -> a':merkle_addr -> vlog_entry_thread
+  | EvictM: a:merkle_addr -> a':merkle_addr -> vlog_entry_thread
+
+(* verifier log entry *)
+type vlog_entry = 
+  | VLogEntry: tid:nat -> e:vlog_entry_thread -> vlog_entry
 
 (* single verifier log *)
-type verifier_log = seq verifier_log_entry
+type vlog = seq vlog_entry
 
 (* index in the verifier log *)
-type vl_index (l:verifier_log) = seq_index l
+type vl_index (l:vlog) = seq_index l
 
-(* verifier state is a subset of merkle_addr, merkle_payloads *)
-type verifier_state = (a:merkle_addr) -> option (merkle_payload_of_addr a)
+(* verifier store is a subset of merkle_addr, merkle_payloads *)
+type vstore = (a:merkle_addr) -> option (merkle_payload_of_addr a)
+
+(* does the store contain address a *)
+let store_contains (store:vstore) (a:merkle_addr) = Some? (store a)
+
+(* lookup the payload of an address in store *)
+let stored_payload (store:vstore) (a:merkle_addr{store_contains store a}):
+  (merkle_payload_of_addr a) = 
+  Some?.v (store a)
+
+(* update the store *)
+let store_update (store:vstore) 
+                 (a:merkle_addr{store_contains store a})
+                 (v:merkle_payload_of_addr a):
+  Tot (store':vstore {store_contains store' a /\ 
+                      stored_payload store' a = v}) = 
+  fun a' -> if a' = a then Some v else store a'
+
+(* per-thread verifier state *)
+noeq type vthread_state = 
+  | VerifierThread: store:vstore -> clk:timestamp -> lk:merkle_addr -> vthread_state
+
+(* get the store of a thread *)
+let thread_store (ts: vthread_state): vstore = VerifierThread?.store ts
+
+(* update the store of a thread *)
+let thread_store_update (ts: vthread_state)
+                        (a:merkle_addr{store_contains (thread_store ts) a})
+                        (v:merkle_payload_of_addr a): 
+  Tot (ts': vthread_state{store_contains (thread_store ts') a /\
+                          stored_payload (thread_store ts') a = v}) = 
+  match ts with
+  | VerifierThread store clk lk -> 
+    VerifierThread (store_update store a v) clk lk
+
+type vglobal_state = 
+  | VerifierGlobal: hadd0:ms_hash_value ->
+           hevict0:ms_hash_value ->
+           hadd1:ms_hash_value ->
+           hevict1:ms_hash_value ->
+           ne:nat -> vglobal_state
+
+(* verifier state aggregated across all verifier threads *)
+noeq type vstate (p:nat) = 
+  | Failed: vstate p
+  | Valid: ts:seq vthread_state{length ts = p} ->  (* thread-specific state *)
+           gs:vglobal_state ->                     (* global state *)
+           vstate p
+
+let verifier_read (#p:nat) (a:addr) (v:payload) 
+                  (tid:nat {tid < p}) 
+                  (vs: vstate p{Valid? vs}): vstate p = 
+  (* thread state *)
+  let ts = index (Valid?.ts vs) tid in
+  (* thread store *)
+  let store = VerifierThread?.store ts in
+  (* merkle addr *)
+  let ma = addr_to_merkle_leaf a in
+  (* check store contains addr *)
+  let optPayload = store ma in
+
+  match optPayload with
+  | None -> Failed
+  | Some v' -> if v = MkLeaf?.value v' then vs 
+               else Failed      
+
+let verifier_write (#p:nat) (a:addr) (v:payload)
+                   (tid:nat {tid < p}) 
+                   (vs: vstate p{Valid? vs}): vstate p = 
+  (* thread state *)
+  let ts = index (Valid?.ts vs) tid in
+  (* thread store *)
+  let store = VerifierThread?.store ts in
+  (* merkle addr *)
+  let ma = addr_to_merkle_leaf a in
+  (* check store contains addr *)
+  let optPayload = store ma in
+
+  match optPayload with
+  | None -> Failed
+  | Some _ -> admit() 
+
+let verifier_step_thread (#p:nat) 
+                         (e:vlog_entry_thread) 
+                         (tid:nat {tid < p}) 
+                         (vs:vstate p{Valid? vs}): vstate p = 
+  // thread state                         
+  let ts = index (Valid?.ts vs) tid in
+  // global state
+  let gs = Valid?.gs vs in
+  // thread store
+  let store = VerifierThread?.store ts in
+  match e with
+  | MemoryOp o -> 
+    (
+    match o with
+    | Read a v -> verifier_read a v tid vs      
+    | Write a v -> admit()
+    )
+  | AddM _ _ _ -> 
+    admit()
+  | EvictM _ _ ->
+    admit()
+
+let verifier_step (#p:nat) (e:vlog_entry) (vs:vstate p): vstate p = 
+  match vs with
+  | Failed -> Failed              // propagate failures
+  | Valid ts gs -> 
+    match e with
+    VLogEntry tid e' ->
+      if tid >= p then  Failed   // invalid thread id       
+      else verifier_step_thread e' tid vs        
+
+(* verify a log from a specified initial state *)
+let rec verifier_aux (#p:nat) (l:vlog) (vs:vstate p): Tot (vstate p)
+  (decreases (length l)) = 
+  let n = length l in
+  if n = 0 then vs
+  else
+    let l' = prefix l (n - 1) in
+    let vs' = verifier_aux l' vs in
+    let e' = index l (n - 1) in
+    verifier_step e' vs'
+
+(* initialize verifier state *)
+let init_vstate (p:nat): vstate p = admit()
+
+let verifier (p:nat) (l:vlog): Tot (vstate p) = 
+  verifier_aux l (init_vstate p)
